solve exercise sheet 4

lean/love04_functional_programming_exercise_sheet.lean
@@ -27,14 +27,19 @@ not strong enough. Start by proving the following generalization (using the
 `induction'` tactic or pattern matching): -/
 
 lemma accurev_eq_reverse_append {α : Type} :
-  ∀as xs : list α, accurev as xs = reverse xs ++ as :=
-sorry
+  ∀as xs : list α, accurev as xs = reverse xs ++ as
+| as []        := by refl
+| as (x :: xs) := by simp [accurev, reverse, accurev_eq_reverse_append (x :: as) xs]
 
 /- 1.2. Derive the desired equation. -/
 
 lemma accurev_eq_reverse {α : Type} (xs : list α) :
   accurev [] xs = reverse xs :=
-sorry
+calc  accurev [] xs
+    = reverse xs ++ [] :
+  by rw accurev_eq_reverse_append
+... = reverse xs :
+  by simp [reverse]
 
 /- 1.3. Prove the following property.
 
@@ -42,7 +47,7 @@ Hint: A one-line inductionless proof is possible. -/
 
 lemma accurev_accurev {α : Type} (xs : list α) :
   accurev [] (accurev [] xs) = xs :=
-sorry
+by simp [accurev_eq_reverse, reverse_reverse]
 
 /- 1.4. Prove the following lemma by structural induction, as a "paper" proof.
 This is a good exercise to develop a deeper understanding of how structural
@@ -67,7 +72,21 @@ not be justified if you think they are obvious (to humans), but you should say
 which key lemmas they depend on. You should be explicit whenever you use a
 function definition or an introduction rule for an inductive predicate. -/
 
--- enter your paper proof here
+/- We show
+    `∀ xs as, accurev as xs = reverse xs ++ as`
+by structural induction on `xs`.
+
+By definition, `accurev as [] = as` and `reverse [] = []`.
+Hence `accurev as [] = as = [] ++ as = reverse [] ++ as`.
+
+Assume `∀ as, accurev as xs = reverse xs ++ as` as induction hypothesis.
+We have
+    `accurev as (x :: xs) = accurev (x :: as) xs` by definition
+                         `= reverse xs ++ (x :: as)` by induction hypothesis
+and
+    `reverse (x :: xs) ++ as = reverse xs ++ [x] ++ as` by definition
+                            `= reverse xs ++ (x :: as)`.
+Hence `accurev as (x :: xs) = reverse (x :: xs) ++ as`. -/
 
 
 /- ## Question 2: Drop and Take
@@ -87,8 +106,10 @@ at the front of a list.
 To avoid unpleasant surprises in the proofs, we recommend that you follow the
 same recursion pattern as for `drop` above. -/
 
-def take {α : Type} : ℕ → list α → list α :=
-sorry
+def take {α : Type} : ℕ → list α → list α
+| 0       xs        := []
+| (_ + 1) []        := []
+| (n + 1) (x :: xs) := x :: (take n xs)
 
 #eval take 0 [3, 7, 11]   -- expected: []
 #eval take 1 [3, 7, 11]   -- expected: [3]
@@ -103,12 +124,14 @@ Notice that they are registered as simplification rules thanks to the `@[simp]`
 attribute. -/
 
 @[simp] lemma drop_nil {α : Type} :
-  ∀n : ℕ, drop n ([] : list α) = [] :=
-sorry
+  ∀n : ℕ, drop n ([] : list α) = []
+| 0       := by refl
+| (_ + 1) := by refl
 
 @[simp] lemma take_nil {α : Type} :
-  ∀n : ℕ, take n ([] : list α) = [] :=
-sorry
+  ∀n : ℕ, take n ([] : list α) = []
+| 0       := by refl
+| (_ + 1) := by refl
 
 /- 2.3. Follow the recursion pattern of `drop` and `take` to prove the
 following lemmas. In other words, for each lemma, there should be three cases,
@@ -122,15 +145,25 @@ Hint: The `refl` tactic might be useful in the third case of `drop_drop`. -/
 lemma drop_drop {α : Type} :
   ∀(m n : ℕ) (xs : list α), drop n (drop m xs) = drop (n + m) xs
 | 0       n xs        := by refl
--- supply the two missing cases here
+| (_ + 1) n []        := by simp
+| (m + 1) n (x :: xs) :=
+  begin
+    simp [drop],
+    simp [drop_drop m n xs],
+    refl,
+  end
 
 lemma take_take {α : Type} :
-  ∀(m : ℕ) (xs : list α), take m (take m xs) = take m xs :=
-sorry
+  ∀(m : ℕ) (xs : list α), take m (take m xs) = take m xs
+| 0       _         := by refl
+| (_ + 1) []        := by refl
+| (n + 1) (x :: xs) := by simp [take, take_take n xs]
 
 lemma take_drop {α : Type} :
-  ∀(n : ℕ) (xs : list α), take n xs ++ drop n xs = xs :=
-sorry
+  ∀(n : ℕ) (xs : list α), take n xs ++ drop n xs = xs
+| 0       _         := by refl
+| (_ + 1) []        := by refl
+| (n + 1) (x :: xs) := by simp [take, drop, take_drop n xs]
 
 
 /- ## Question 3: A Type of λ-Terms
@@ -142,14 +175,19 @@ by the following context-free grammar:
            | 'lam' string term   -- λ-expression (e.g., `λx, t`)
            | 'app' term term     -- application (e.g., `t u`) -/
 
--- enter your definition here
+inductive term : Type
+| var : string → term
+| lam : string → term → term
+| app : term → term → term
 
 /- 3.2. Register a textual representation of the type `term` as an instance of
 the `has_repr` type class. Make sure to supply enough parentheses to guarantee
 that the output is unambiguous. -/
 
 def term.repr : term → string
--- enter your answer here
+| (term.var x)   := x
+| (term.lam x t) := "(λ " ++ x ++ ", " ++ term.repr t ++ ")"
+| (term.app t u) := "(" ++ term.repr t ++ " " ++ term.repr u ++ ")"
 
 @[instance] def term.has_repr : has_repr term :=
 { repr := term.repr }
